Moved reprogramming to prom

Reprogramming.ec
@@ -1,6 +1,5 @@
-require import AllCore List Int Distr RealExp SmtMap FinType StdOrder StdBigop.
+require import AllCore List Int Distr RealExp SmtMap FinType StdOrder StdBigop PROM.
 (*---*) import Bigreal.BRA Bigreal RField RealOrder.
-require (*--*) ROM.
 
 type in_t.
 
@@ -9,14 +8,13 @@ type out_t.
 type pT = in_t distr.
 
 clone import FinType as FT_In with
-  type t <- in_t.
+  type t = in_t.
 
 op [lossless] dout : out_t distr.
 
 const p_max_bound : real.
 
-(*** TODO: Rewrite using PROM ***)
-clone import ROM as ROM_ with
+clone import FullRO as ROM_ with
   type in_t <- in_t,
   type out_t <- out_t,
   op dout <- fun _ => dout,
@@ -25,8 +23,8 @@ clone import ROM as ROM_ with
   
   proof *.
  
-clone import ROM_.LazyEager as LE with 
-  theory FinType <- FT_In
+clone import FinEager as LE with 
+  theory FinFrom <- FT_In
   
   proof *.
 
@@ -39,15 +37,14 @@ clone import ROM_.LazyEager as LE with
 theory Adaptive.
   
 module type Oracleip_t = {
-  include Oracle
-  proc set(x : in_t, y : out_t) : unit
+  include RO [init, get, set]
 }.
 
 module type Oraclep_t = {
   include Oracleip_t [-init]
 }.
 
-module O_Programmable(O : POracle) : Oraclep_t = {
+module O_Programmable(O : RO) : Oraclep_t = {
    var prog_list : (in_t * out_t) list  
    var ch : int
 
@@ -56,11 +53,11 @@ module O_Programmable(O : POracle) : Oraclep_t = {
      ch <- 0;
    }
 
-  proc o(x : in_t) : out_t = {
+  proc get(x : in_t) : out_t = {
     var r,c : out_t;
     var tmp : out_t option;
 
-    r <@ O.o(x);
+    r <@ O.get(x);
 
     ch <- ch + 1; 
     tmp <- assoc prog_list x;
@@ -82,7 +79,6 @@ module type Oracleir_t = {
 module type Oracler_t = {
   include Oracleir_t [-init]
 }.
-
 
 module O_Reprogrammer(O : Oraclep_t) : Oracler_t = {
   var ctr : int
@@ -114,10 +110,10 @@ module O_Reprogrammer(O : Oraclep_t) : Oracler_t = {
 }.
 
 module type Adv_INDRepro(O : Oraclep_t, OR : Oracler_t) = {
-  proc distinguish() : bool {O.o, OR.repro}
+  proc distinguish() : bool {O.get, OR.repro}
 }.
 
-module IND_Repro(O : Oracle, A : Adv_INDRepro) = {
+module IND_Repro(O : RO, A : Adv_INDRepro) = {
   module OP = O_Programmable(O)
   module OR = O_Reprogrammer(OP)
  
@@ -137,7 +133,7 @@ module IND_Repro(O : Oracle, A : Adv_INDRepro) = {
 
 section.
 
-declare module A <: Adv_INDRepro {-IND_Repro, -ERO, -Lazy.LRO}.
+declare module A <: Adv_INDRepro {-IND_Repro, -FunRO, -RO, -FRO}.
 
 declare const rep_ctr : {int | 0 <= rep_ctr } as ge0_repctr.
 declare const query_ctr : {int | 0 <= query_ctr } as ge0_queryctr.
@@ -149,23 +145,23 @@ local module Bad = {
   var i  : int
 }.
 
-local module O_Programmable1 (O : POracle) : Oracleip_t = {
-  include var O_Programmable(O) [-o]
+local module O_Programmable1 (O : RO) : Oracleip_t = {
+  include var O_Programmable(O) [-get]
   import var Bad
  
-  proc o(x : in_t): out_t = {
+  proc get(x : in_t): out_t = {
     var r, c : out_t;
     var tmp : out_t option;
 
     c <- witness;
     if (co < query_ctr) { 
-      r <@ O.o(x);
+      r <@ O.get(x);
       tmp <- assoc prog_list x;
       c <- if tmp = None then r else oget tmp;
       co <- co + 1;
     } else {
       bad <- true;
-      r <@ O.o(x);
+      r <@ O.get(x);
       tmp <- assoc prog_list x;
       c <- if tmp = None then r else oget tmp;      
       co <- co + 1;
@@ -178,17 +174,17 @@ local module O_Programmable1 (O : POracle) : Oracleip_t = {
 
 }.
 
-local module O_Programmable2 (O: POracle) : Oracleip_t = {
-  include var O_Programmable(O) [-o]
+local module O_Programmable2 (O: RO) : Oracleip_t = {
+  include var O_Programmable(O) [-get]
   import var Bad
  
-  proc o(x : in_t): out_t = {
+  proc get(x : in_t): out_t = {
     var r, c : out_t;
     var tmp : out_t option;
 
     c <- witness;
     if (co < query_ctr) { 
-      r <@ O.o(x);
+      r <@ O.get(x);
       tmp <- assoc prog_list x;
       c <- if tmp = None then r else oget tmp;
       co <- co + 1;
@@ -203,17 +199,17 @@ local module O_Programmable2 (O: POracle) : Oracleip_t = {
 
 }.
 
-local module O_Programmable2S (O: POracle) : Oracleip_t = {
-  include var O_Programmable(O) [-o]
+local module O_Programmable2S (O: RO) : Oracleip_t = {
+  include var O_Programmable(O) [-get]
   import var Bad
 
-  proc o(x : in_t): out_t = {
+  proc get(x : in_t): out_t = {
     var r, c : out_t;
     var tmp : out_t option;
 
     c <- witness;
     if (co < query_ctr) { 
-      r <@ O.o(x);
+      r <@ O.get(x);
       tmp <- assoc prog_list x;
       c <- if tmp = None then r else oget tmp;
       co <- co + 1;
@@ -287,7 +283,7 @@ local module O_Reprogrammer2(O: Oraclep_t) : Oracleir_t = {
   }
 }.
 
-local module IND_Repro1 (O: Oracle, A: Adv_INDRepro) = {
+local module IND_Repro1 (O: RO, A: Adv_INDRepro) = {
   import var Bad
   
   module OP = O_Programmable1(O)
@@ -308,7 +304,7 @@ local module IND_Repro1 (O: Oracle, A: Adv_INDRepro) = {
   } 
 }.
 
-local module IND_Repro2 (O: Oracle, A: Adv_INDRepro) = {
+local module IND_Repro2 (O: RO, A: Adv_INDRepro) = {
   import var Bad
   
   module OP = O_Programmable2(O)
@@ -330,13 +326,13 @@ local module IND_Repro2 (O: Oracle, A: Adv_INDRepro) = {
 }.
 
 local lemma Pr_count &m (b : bool) : 
-     hoare[ A(O_Programmable(ERO),O_Reprogrammer(O_Programmable(ERO))).distinguish : 
+     hoare[ A(O_Programmable(FunRO),O_Reprogrammer(O_Programmable(FunRO))).distinguish : 
              O_Programmable.ch = 0 /\ O_Reprogrammer.ctr = 0 /\ O_Reprogrammer.se 
              ==> O_Programmable.ch <= query_ctr /\ 
              O_Reprogrammer.ctr <= rep_ctr /\ O_Reprogrammer.se] 
-  => Pr[IND_Repro(ERO, A).main(b) @ &m : res] 
+  => Pr[IND_Repro(FunRO, A).main(b) @ &m : res] 
      = 
-     Pr[IND_Repro(ERO,A).main(b) @ &m : res /\ O_Programmable.ch <= query_ctr /\ O_Reprogrammer.ctr <= rep_ctr /\ O_Reprogrammer.se].
+     Pr[IND_Repro(FunRO,A).main(b) @ &m : res /\ O_Programmable.ch <= query_ctr /\ O_Reprogrammer.ctr <= rep_ctr /\ O_Reprogrammer.se].
 proof.
 move=> hhoare.
 byequiv => //.
@@ -347,12 +343,12 @@ by proc; call hhoare; inline *; auto => /=.
 qed.
 
 local lemma Pr_Game_Game1 &m b : 
-  Pr[IND_Repro(ERO,A).main(b) @ &m:res /\  O_Programmable.ch <= query_ctr /\ O_Reprogrammer.ctr <= rep_ctr /\ O_Reprogrammer.se] =
-  Pr[IND_Repro1(ERO,A).main(b) @ &m:res /\  O_Programmable.ch <= query_ctr /\ O_Reprogrammer.ctr <= rep_ctr /\ O_Reprogrammer.se].
+  Pr[IND_Repro(FunRO,A).main(b) @ &m:res /\  O_Programmable.ch <= query_ctr /\ O_Reprogrammer.ctr <= rep_ctr /\ O_Reprogrammer.se] =
+  Pr[IND_Repro1(FunRO,A).main(b) @ &m:res /\  O_Programmable.ch <= query_ctr /\ O_Reprogrammer.ctr <= rep_ctr /\ O_Reprogrammer.se].
 proof.
 byequiv => //.
 proc.
-call (:    ={glob ERO,  glob O_Reprogrammer, glob O_Programmable} 
+call (:    ={glob FunRO,  glob O_Reprogrammer, glob O_Programmable} 
        /\ ((O_Reprogrammer.ctr, O_Programmable.ch) = (Bad.cr,Bad.co)){2}).
 + proc.
   case (Bad.co{2} < query_ctr). 
@@ -370,25 +366,22 @@ call (:    ={glob ERO,  glob O_Reprogrammer, glob O_Programmable}
     by wp => />; sim.
   rcondf{2} 2; 1: by auto. 
   by wp => />; sim.
-inline *.
-wp.
-swap{2} [1..3] 3.
-by wp => />; sim.
+by inline *;auto.
 qed.
 
 local lemma Pr_Game1_Game2 &m b: 
-  Pr[IND_Repro1(ERO,A).main(b) @ &m: res /\ O_Programmable.ch <= query_ctr /\ O_Reprogrammer.ctr <= rep_ctr /\ O_Reprogrammer.se] =
-  Pr[IND_Repro2(ERO,A).main(b) @ &m: res /\ O_Programmable.ch <= query_ctr /\ O_Reprogrammer.ctr <= rep_ctr /\ O_Reprogrammer.se].
+  Pr[IND_Repro1(FunRO,A).main(b) @ &m: res /\ O_Programmable.ch <= query_ctr /\ O_Reprogrammer.ctr <= rep_ctr /\ O_Reprogrammer.se] =
+  Pr[IND_Repro2(FunRO,A).main(b) @ &m: res /\ O_Programmable.ch <= query_ctr /\ O_Reprogrammer.ctr <= rep_ctr /\ O_Reprogrammer.se].
 proof.
 have: 
-  `| Pr[IND_Repro1(ERO,A).main(b) @ &m: res /\ O_Programmable.ch <= query_ctr /\ O_Reprogrammer.ctr <= rep_ctr /\ O_Reprogrammer.se] -
-     Pr[IND_Repro2(ERO,A).main(b) @ &m: res /\ O_Programmable.ch <= query_ctr /\ O_Reprogrammer.ctr <= rep_ctr /\ O_Reprogrammer.se] | 
+  `| Pr[IND_Repro1(FunRO,A).main(b) @ &m: res /\ O_Programmable.ch <= query_ctr /\ O_Reprogrammer.ctr <= rep_ctr /\ O_Reprogrammer.se] -
+     Pr[IND_Repro2(FunRO,A).main(b) @ &m: res /\ O_Programmable.ch <= query_ctr /\ O_Reprogrammer.ctr <= rep_ctr /\ O_Reprogrammer.se] | 
   <=
-  RealOrder.maxr Pr[IND_Repro1(ERO,A).main(b) @ &m: (res /\ O_Programmable.ch <= query_ctr /\ O_Reprogrammer.ctr <= rep_ctr /\ O_Reprogrammer.se) /\ Bad.bad] 
-                 Pr[IND_Repro2(ERO,A).main(b) @ &m: (res /\ O_Programmable.ch <= query_ctr /\ O_Reprogrammer.ctr <= rep_ctr /\ O_Reprogrammer.se) /\ Bad.bad].
+  RealOrder.maxr Pr[IND_Repro1(FunRO,A).main(b) @ &m: (res /\ O_Programmable.ch <= query_ctr /\ O_Reprogrammer.ctr <= rep_ctr /\ O_Reprogrammer.se) /\ Bad.bad] 
+                 Pr[IND_Repro2(FunRO,A).main(b) @ &m: (res /\ O_Programmable.ch <= query_ctr /\ O_Reprogrammer.ctr <= rep_ctr /\ O_Reprogrammer.se) /\ Bad.bad].
 + byupto.
 have ->: 
-  Pr[IND_Repro1(ERO, A).main(b) @ &m : (res /\ O_Programmable.ch <= query_ctr /\ O_Reprogrammer.ctr <= rep_ctr /\ O_Reprogrammer.se) /\ Bad.bad] 
+  Pr[IND_Repro1(FunRO, A).main(b) @ &m : (res /\ O_Programmable.ch <= query_ctr /\ O_Reprogrammer.ctr <= rep_ctr /\ O_Reprogrammer.se) /\ Bad.bad] 
   = 
   0%r.
 + byphoare => //.
@@ -401,9 +394,9 @@ have ->:
   + proc; sp; wp; if; auto. 
     - by conseq (: _ ==> true); auto => /#.
     by swap 1 2; wp; conseq (: _ ==> true); auto => /#.
-  inline *; swap [1..3] 3; auto; conseq (: _ ==> true) => //= /#.
+  by inline *; auto => /#.
 have -> /#: 
-  Pr[IND_Repro2(ERO, A).main(b) @ &m : (res /\ O_Programmable.ch <= query_ctr /\ O_Reprogrammer.ctr <= rep_ctr /\ O_Reprogrammer.se) /\ Bad.bad] 
+  Pr[IND_Repro2(FunRO, A).main(b) @ &m : (res /\ O_Programmable.ch <= query_ctr /\ O_Reprogrammer.ctr <= rep_ctr /\ O_Reprogrammer.se) /\ Bad.bad] 
   = 
   0%r.
 byphoare => //.
@@ -415,11 +408,11 @@ call (:   Bad.cr <= O_Reprogrammer.ctr
 + by proc; sp; wp; if; auto; 1: call (: true); auto => /#.
 + proc; sp; wp; if; auto; 2: smt().
   by conseq (: _ ==> true); auto => /#.
-by inline *; swap [1..3] 3; auto; conseq (: _ ==> true) => //= /#.
+by inline *; auto => /#.
 qed.
 
 local module O_Reprogrammer2i : Oracleir_t = {
-  include var O_Reprogrammer(O_Programmable2S(ERO)) [-repro]
+  include var O_Reprogrammer(O_Programmable2S(FunRO)) [-repro]
   import var Bad
 
   proc repro(p: pT) : in_t = {
@@ -433,7 +426,7 @@ local module O_Reprogrammer2i : Oracleir_t = {
       x <$ p;
       if (i <= cr) {
         y <$ dout;
-        O_Programmable2(ERO).set(x,y);
+        O_Programmable2(FunRO).set(x,y);
       }
       cr <- cr + 1;
     } 
@@ -447,7 +440,7 @@ local module O_Reprogrammer2i : Oracleir_t = {
 local module Hi = {
   import var Bad
   
-  module OP = O_Programmable2S(ERO)
+  module OP = O_Programmable2S(FunRO)
   module OR = O_Reprogrammer2i
  
   proc main (i0: int) : bool = {
@@ -455,7 +448,7 @@ local module Hi = {
     
     bad <- false; cr <- 0; co <- 0; i <- i0;
     
-    ERO.init();
+    FunRO.init();
     OP.init();
     OR.init(false);
     
@@ -466,33 +459,33 @@ local module Hi = {
 }.
 
 local lemma Hi_true &m : 
-  Pr[IND_Repro2(ERO, A).main(true) @ &m : res /\ O_Programmable.ch <= query_ctr /\ O_Reprogrammer.ctr <= rep_ctr /\ O_Reprogrammer.se]
+  Pr[IND_Repro2(FunRO, A).main(true) @ &m : res /\ O_Programmable.ch <= query_ctr /\ O_Reprogrammer.ctr <= rep_ctr /\ O_Reprogrammer.se]
   = 
   Pr[Hi.main(0) @ &m : res].
 proof.
 byequiv => //.
 proc.
-call (:   ={glob O_Programmable, O_Reprogrammer.se, O_Reprogrammer.ctr, ERO.m, Bad.cr, Bad.co} 
+call (:   ={glob O_Programmable, O_Reprogrammer.se, O_Reprogrammer.ctr, FunRO.f, Bad.cr, Bad.co} 
        /\ O_Reprogrammer.b{1} 
        /\ (Bad.i <= Bad.cr){2}).
 + by sim />.
 + proc. 
   seq 2 2 : (#pre /\ ={x}); 1: by auto.
   wp; if; auto.
-  conseq (: ={glob O_Programmable, O_Reprogrammer.se, O_Reprogrammer.ctr, ERO.m, x}); 1: smt().
+  conseq (: ={glob O_Programmable, O_Reprogrammer.se, O_Reprogrammer.ctr, FunRO.f, x}); 1: smt().
   seq 1 1 : (#pre); 1: by sim />.
   by if; auto; sim.
 by inline *; swap{1} [1 ..3] 3; swap{2} [1 ..4] 3; auto; sim />.
 qed.
 
 local lemma Hi_false &m : 
-  Pr[IND_Repro2(ERO, A).main(false) @ &m : res /\ O_Programmable.ch <= query_ctr /\ O_Reprogrammer.ctr <= rep_ctr /\ O_Reprogrammer.se]
+  Pr[IND_Repro2(FunRO, A).main(false) @ &m : res /\ O_Programmable.ch <= query_ctr /\ O_Reprogrammer.ctr <= rep_ctr /\ O_Reprogrammer.se]
   = 
   Pr[Hi.main(rep_ctr) @ &m : res].
 proof.
 byequiv => //.
 proc.
-call (:   ={glob O_Programmable, O_Reprogrammer.se, O_Reprogrammer.ctr, ERO.m, Bad.cr, Bad.co} 
+call (:   ={glob O_Programmable, O_Reprogrammer.se, O_Reprogrammer.ctr, FunRO.f, Bad.cr, Bad.co} 
        /\ !O_Reprogrammer.b{1} 
        /\ (Bad.i = rep_ctr){2}).
 + by sim />.
@@ -504,7 +497,7 @@ call (:   ={glob O_Programmable, O_Reprogrammer.se, O_Reprogrammer.ctr, ERO.m, B
 inline *; swap{1} [1 ..3] 3; swap{2} [1 ..4] 3; auto; sim />.
 qed.
 
-local module O_Reprogrammer2i1 (O: POracle) : Oracleir_t = {
+local module O_Reprogrammer2i1 (O: RO) : Oracleir_t = {
   import var Bad
 
   include var O_Reprogrammer(O_Programmable2S(O)) [-repro]
@@ -526,7 +519,7 @@ local module O_Reprogrammer2i1 (O: POracle) : Oracleir_t = {
       } else { 
         if (i = cr) {
           x_ <- x;
-          y <@ O.o(x);
+          y <@ O.get(x);
         } 
       } 
       cr <- cr + 1;
@@ -538,13 +531,13 @@ local module O_Reprogrammer2i1 (O: POracle) : Oracleir_t = {
   }
 }.
 
-local module Hi1 (O:POracle) = {
+local module Hi1 (O:RO) = {
   import var Bad
   
   module OP = O_Programmable2S(O)
   module OR = O_Reprogrammer2i1(O)
  
-  proc run (i0: int) : bool = {
+  proc distinguish (i0: int) : bool = {
     var b' : bool;
  
     bad <- false;  cr <- 0; co <- 0; i <- i0;
@@ -560,12 +553,12 @@ local module Hi1 (O:POracle) = {
 local lemma Hip1_Hi1 &m i_ : 
   Pr[Hi.main(i_ + 1) @ &m : res] 
   = 
-  Pr[Exp(ERO, Hi1).main(i_) @ &m : res].
+  Pr[MainD(Hi1,FunRO).distinguish(i_) @ &m : res].
 proof.
 byequiv => //. 
 proc. 
 inline *; wp.
-call (:   ={ERO.m, glob O_Programmable, glob O_Reprogrammer, Bad.cr, Bad.co} 
+call (:   ={FunRO.f, glob O_Programmable, glob O_Reprogrammer, Bad.cr, Bad.co} 
        /\ Bad.i{1} = Bad.i{2} + 1).
 + by sim />.
 + proc; wp; conseq />.
@@ -577,18 +570,20 @@ call (:   ={ERO.m, glob O_Programmable, glob O_Reprogrammer, Bad.cr, Bad.co}
 by swap{1} [1..4] 3; auto; sim />.
 qed.
 
-local lemma Hi1_ERO_LRO  &m i_ : 
-  Pr[Exp(ERO,Hi1).main(i_) @ &m : res] 
+local lemma Hi1_FunRO_RO  &m i_ : 
+  Pr[MainD(Hi1,FunRO).distinguish(i_) @ &m : res] 
   =
-  Pr[Exp(Lazy.LRO,Hi1).main(i_) @ &m : res].
+  Pr[MainD(Hi1,RO).distinguish(i_) @ &m : res].
 proof.
-byequiv (: ={glob Hi1, arg} ==> ={res}) => //; symmetry.
-conseq (eq_eager_sampling Hi1 _) => // *; apply dout_ll.
+have <- : Pr[MainD(Hi1, FinRO).distinguish(i_) @ &m : res] = 
+          Pr[MainD(Hi1, FunRO).distinguish(i_) @ &m : res]
+  by  apply (pr_FinRO_FunRO_D _ Hi1 &m i_ (fun b => b));smt(dout_ll).
+by rewrite (pr_RO_FinRO_D _ Hi1 &m i_ (fun b => b));smt(dout_ll).
 qed.
 
 local module O_Reprogrammer2i2 : Oracleir_t = {
   import var Bad
-  include var O_Reprogrammer(O_Programmable2S(Lazy.LRO)) [-repro]
+  include var O_Reprogrammer(O_Programmable2S(RO)) [-repro]
   
   var x_ : in_t
 
@@ -603,14 +598,14 @@ local module O_Reprogrammer2i2 : Oracleir_t = {
       x <$ p;
       if (i + 1 <= cr) {
         y <$ dout;
-        O_Programmable2S(Lazy.LRO).set(x,y);
-      } else { if (i = cr /\ fsize Lazy.LRO.m <= query_ctr) {
+        O_Programmable2S(RO).set(x,y);
+      } else { if (i = cr /\ fsize RO.m <= query_ctr) {
         x_ <- x;
-        if (! x \in Lazy.LRO.m) {
-          y <@ Lazy.LRO.o(x);
+        if (! x \in RO.m) {
+          y <@ RO.get(x);
         } else { 
           bad <- true;
-          y <@ Lazy.LRO.o(x);          
+          y <@ RO.get(x);          
         }
       } } 
       cr <- cr + 1;
@@ -625,7 +620,7 @@ local module O_Reprogrammer2i2 : Oracleir_t = {
 local module Hi2 = {
   import var Bad
   
-  module OP = O_Programmable2S(Lazy.LRO)
+  module OP = O_Programmable2S(RO)
   module OR = O_Reprogrammer2i2
  
   proc run (i0: int) : bool = {
@@ -633,7 +628,7 @@ local module Hi2 = {
     
     bad <- false;  cr <- 0; co <- 0; i <- i0;
     
-    Lazy.LRO.init();
+    RO.init();
     OP.init();
     OR.init(false);
     
@@ -645,7 +640,7 @@ local module Hi2 = {
 
 local module O_Reprogrammer2i3 : Oracleir_t = {
   import var Bad
-  include var O_Reprogrammer(O_Programmable2S(Lazy.LRO)) [-repro]
+  include var O_Reprogrammer(O_Programmable2S(RO)) [-repro]
 
   proc repro(p: pT) : in_t = {
     var x : in_t;
@@ -658,15 +653,15 @@ local module O_Reprogrammer2i3 : Oracleir_t = {
       x <$ p;
       if (i + 1 <= cr) {
         y <$ dout;
-        O_Programmable2S(Lazy.LRO).set(x,y);
-      } else { if (i = cr /\ fsize Lazy.LRO.m <= query_ctr) {
+        O_Programmable2S(RO).set(x,y);
+      } else { if (i = cr /\ fsize RO.m <= query_ctr) {
         O_Reprogrammer2i2.x_ <- x;
-        if (! x \in Lazy.LRO.m) {
-          y <@ Lazy.LRO.o(x);
+        if (! x \in RO.m) {
+          y <@ RO.get(x);
         } else { 
           bad <- true;
-          Lazy.LRO.m <- rem Lazy.LRO.m x;
-          y <@ Lazy.LRO.o(x); 
+          RO.m <- rem RO.m x;
+          y <@ RO.get(x); 
         }
       } } 
       cr <- cr + 1;
@@ -681,7 +676,7 @@ local module O_Reprogrammer2i3 : Oracleir_t = {
 local module Hi3 = {
   import var Bad
   
-  module OP = O_Programmable2S(Lazy.LRO)
+  module OP = O_Programmable2S(RO)
   module OR = O_Reprogrammer2i3
  
   proc run (i0: int) : bool = {
@@ -689,7 +684,7 @@ local module Hi3 = {
     
     bad <- false;  cr <- 0; co <- 0; i <- i0;
   
-    Lazy.LRO.init();
+    RO.init();
     OP.init();
     OR.init(false);
   
@@ -699,13 +694,13 @@ local module Hi3 = {
   } 
 }.
 
-local lemma Hi1_LRO_Hi2  &m i_ : Pr[ Exp(Lazy.LRO,Hi1).main(i_) @ &m : res] = Pr[Hi2.run(i_) @ &m : res].
+local lemma Hi1_LRO_Hi2  &m i_ : Pr[ MainD(Hi1,RO).distinguish(i_) @ &m : res] = Pr[Hi2.run(i_) @ &m : res].
 proof.
 byequiv => //.
 proc. 
 inline *; wp.
-call (:   ={ Lazy.LRO.m, glob O_Programmable, glob O_Reprogrammer, Bad.cr, Bad.co, Bad.i} 
-       /\ (Bad.cr <= Bad.i => fsize Lazy.LRO.m <= Bad.co <= query_ctr){1}); last first.
+call (:   ={ RO.m, glob O_Programmable, glob O_Reprogrammer, Bad.cr, Bad.co, Bad.i} 
+       /\ (Bad.cr <= Bad.i => fsize RO.m <= Bad.co <= query_ctr){1}); last first.
 + by auto => />; rewrite fsize_empty ge0_queryctr.
 + by proc; sp; inline *; if; auto => /> &2 3? r *; rewrite fsize_set /b2i => /> /#.
 proc. 
@@ -719,7 +714,7 @@ if => //.
 wp. 
 if => //; 1: smt().
 + sp 1 1. 
-  conseq (: _ ==> ={Lazy.LRO.m}); [smt() | if{2}; sim].
+  conseq (: _ ==> ={RO.m}); [smt() | if{2}; sim].
 by auto => /#.
 qed.
 
@@ -738,7 +733,7 @@ fel 4
     1 
     Bad.bad
     [O_Reprogrammer2i2.repro :   ((if p_max p <= p_max_bound then O_Reprogrammer.se else false) 
-                              /\ Bad.cr < rep_ctr /\ Bad.i = Bad.cr /\ fsize Lazy.LRO.m <= query_ctr)] => //.
+                              /\ Bad.cr < rep_ctr /\ Bad.i = Bad.cr /\ fsize RO.m <= query_ctr)] => //.
 + by rewrite sumri_const.
 + smt().
 + auto => /> /#.
@@ -746,13 +741,13 @@ fel 4
   rcondt ^if; 1: by auto.
   rcondf ^if; 1: by auto => /#.
   rcondt ^if; 1: by auto.
-  wp; seq 3 : (x \in Lazy.LRO.m) (query_ctr%r * p_max_bound) 1%r _ 0%r (!Bad.bad) => //.
+  wp; seq 3 : (x \in RO.m) (query_ctr%r * p_max_bound) 1%r _ 0%r (!Bad.bad) => //.
   + by auto.
-  + rnd (fun p => p \in Lazy.LRO.m); auto.
+  + rnd (fun p => p \in RO.m); auto.
     move=> &hr /> _ _ _ hmax _ _ hsz.
-    apply (ler_trans (mu p{hr} (fun (p0 : in_t ) => exists x, dom Lazy.LRO.m{hr} x /\ x = p0))).
+    apply (ler_trans (mu p{hr} (fun (p0 : in_t ) => exists x, dom RO.m{hr} x /\ x = p0))).
     + by apply mu_le => /> x0 *; exists x0.
-    apply (ler_trans ((fsize Lazy.LRO.m{hr})%r * p_max_bound)).
+    apply (ler_trans ((fsize RO.m{hr})%r * p_max_bound)).
     apply: Mu_mem.mu_mem_le_fsize.
     + move=> x hx /=; apply: ler_trans hmax; move: (pmax_upper_bound p{hr} x) => /#.
     by apply ler_wpmul2r; smt(pmax_ge0). 
@@ -762,7 +757,7 @@ fel 4
   rcondt ^if; 1: by auto.
   by wp; conseq (: _ ==> true) => //; smt().
 move=> b c; proc.
-seq 2: (   ! (O_Reprogrammer.se /\ Bad.cr < rep_ctr /\ Bad.i = Bad.cr /\ FSet.card (fdom Lazy.LRO.m) <= query_ctr) 
+seq 2: (   ! (O_Reprogrammer.se /\ Bad.cr < rep_ctr /\ Bad.i = Bad.cr /\ FSet.card (fdom RO.m) <= query_ctr) 
         /\ Bad.bad = b 
         /\ b2i (Bad.i < Bad.cr) = c); 1: by auto.
 wp; if; last by auto.
@@ -784,7 +779,7 @@ fel 4
     1 
     Bad.bad
     [O_Reprogrammer2i3.repro :   ((if p_max p <= p_max_bound then O_Reprogrammer.se else false) 
-                              /\ Bad.cr < rep_ctr /\ Bad.i = Bad.cr /\ fsize Lazy.LRO.m <= query_ctr)] => //.
+                              /\ Bad.cr < rep_ctr /\ Bad.i = Bad.cr /\ fsize RO.m <= query_ctr)] => //.
 + by rewrite sumri_const.
 + smt().
 + auto => /> /#.
@@ -792,13 +787,13 @@ fel 4
   rcondt ^if; 1: by auto.
   rcondf ^if; 1: by auto => /#.
   rcondt ^if; 1: by auto.
-  wp; seq 3 : (x \in Lazy.LRO.m) (query_ctr%r * p_max_bound) 1%r _ 0%r (!Bad.bad) => //.
+  wp; seq 3 : (x \in RO.m) (query_ctr%r * p_max_bound) 1%r _ 0%r (!Bad.bad) => //.
   + by auto.
   + rnd; auto.
     move=> &hr /> _ _ _ hmax _ _ hsz.
-    apply (ler_trans (mu p{hr} (fun (p0 : in_t) => exists x, dom Lazy.LRO.m{hr} x /\ x = p0))).
+    apply (ler_trans (mu p{hr} (fun (p0 : in_t) => exists x, dom RO.m{hr} x /\ x = p0))).
     + by apply mu_le => /> x0 *; exists x0.
-    apply (ler_trans ((fsize Lazy.LRO.m{hr})%r * p_max_bound)).
+    apply (ler_trans ((fsize RO.m{hr})%r * p_max_bound)).
     apply: Mu_mem.mu_mem_le_fsize.
     + by move=> x hx /=; apply: ler_trans hmax;  move: (pmax_upper_bound p{hr} x) => /#.
     by apply ler_wpmul2r; smt(pmax_ge0). 
@@ -809,7 +804,7 @@ fel 4
   by wp; conseq (: _ ==> true) => //; smt().
 move=> b c. 
 proc.
-seq 2: (! (O_Reprogrammer.se /\ Bad.cr < rep_ctr /\ Bad.i = Bad.cr /\ FSet.card (fdom Lazy.LRO.m) <= query_ctr) /\
+seq 2: (! (O_Reprogrammer.se /\ Bad.cr < rep_ctr /\ Bad.i = Bad.cr /\ FSet.card (fdom RO.m) <= query_ctr) /\
              Bad.bad = b /\ b2i (Bad.i < Bad.cr) = c); 1: by auto.
 wp; if; last by auto.
 seq 1 : (#pre); 1: by auto.
@@ -817,7 +812,7 @@ wp; if; 1: by conseq (: _ ==> true) => // /#.
 by rcondf ^if; auto => /#.
 qed.
 
-local module O_Reprogrammer2i4 (O: POracle) : Oracleir_t = {
+local module O_Reprogrammer2i4 (O: RO) : Oracleir_t = {
   import var Bad
   include var O_Reprogrammer(O_Programmable2S(O)) [-repro]
   
@@ -845,13 +840,13 @@ local module O_Reprogrammer2i4 (O: POracle) : Oracleir_t = {
   }
 }.
 
-local module Hi4 (O:POracle) = {
+local module Hi4 (O:RO) = {
   import var Bad
   
   module OP = O_Programmable2S(O)
   module OR = O_Reprogrammer2i4(O)
  
-  proc run (i0: int) : bool = {
+  proc distinguish (i0: int) : bool = {
     var b' : bool;
     
     bad <- false;  cr <- 0; co <- 0; i <- i0;
@@ -869,7 +864,7 @@ local lemma Hi3_Hi4 &m i_:
      0 <= i_ 
   => Pr[Hi3.run(i_) @ &m : res] 
      = 
-     Pr[Exp(Lazy.LRO, Hi4).main(i_) @ &m : res].
+     Pr[MainD(Hi4,RO).distinguish(i_) @ &m : res].
 proof.
 move=> hi. 
 byequiv => //. 
@@ -877,12 +872,12 @@ proc.
 inline *; wp.
 call (:   ={O_Programmable.ch, glob O_Reprogrammer, Bad.i, Bad.cr, Bad.co} 
        /\ if (Bad.cr <= Bad.i){1} 
-          then    ={Lazy.LRO.m, O_Programmable.prog_list} 
+          then    ={RO.m, O_Programmable.prog_list} 
                /\ O_Programmable.prog_list{1} = [] 
-               /\ (fsize Lazy.LRO.m <= Bad.co <= query_ctr){1}
-          else    ((O_Reprogrammer2i2.x_ \in Lazy.LRO.m){1} 
-               /\ O_Programmable.prog_list{2} = (rcons O_Programmable.prog_list (O_Reprogrammer2i2.x_, oget Lazy.LRO.m.[O_Reprogrammer2i2.x_])){1} 
-               /\ eq_except (pred1 O_Reprogrammer2i2.x_{1}) Lazy.LRO.m{1} Lazy.LRO.m{2})).
+               /\ (fsize RO.m <= Bad.co <= query_ctr){1}
+          else    ((O_Reprogrammer2i2.x_ \in RO.m){1} 
+               /\ O_Programmable.prog_list{2} = (rcons O_Programmable.prog_list (O_Reprogrammer2i2.x_, oget RO.m.[O_Reprogrammer2i2.x_])){1} 
+               /\ eq_except (pred1 O_Reprogrammer2i2.x_{1}) RO.m{1} RO.m{2})).
 + proc.
   sp; wp; if => //.
   inline *; auto => |> &1 &2. 
@@ -905,20 +900,25 @@ call (:   ={O_Programmable.ch, glob O_Reprogrammer, Bad.i, Bad.cr, Bad.co}
 by auto => />; rewrite fsize_empty ge0_queryctr.
 qed.
 
-local lemma Hi4_LRO_ERO &m i_: 
-  Pr[Exp(Lazy.LRO, Hi4).main(i_) @ &m : res] 
+local lemma Hi4_RO_FunRO &m i_: 
+  Pr[MainD(Hi4,RO).distinguish(i_) @ &m : res] 
   = 
-  Pr[Exp(ERO, Hi4).main(i_) @ &m : res].
+  Pr[MainD(Hi4,FunRO).distinguish(i_) @ &m : res].
 proof.
-byequiv (: ={glob Hi4, arg} ==> ={res}) => //.
-by conseq (eq_eager_sampling Hi4 _) => // *; apply dout_ll.
+have <- : Pr[MainD(Hi4, FinRO).distinguish(i_) @ &m : res] = 
+          Pr[MainD(Hi4, FunRO).distinguish(i_) @ &m : res]
+  by  apply (pr_FinRO_FunRO_D _ Hi4 &m i_ (fun b => b));smt(dout_ll).
+by rewrite (pr_RO_FinRO_D _ Hi4 &m i_ (fun b => b));smt(dout_ll).
 qed.
 
 local lemma Hi4_Hi &m i_ : 
-  Pr[Exp(ERO, Hi4).main(i_) @ &m : res] 
+  Pr[MainD(Hi4,FunRO).distinguish(i_) @ &m : res] 
   = 
   Pr[Hi.main(i_) @ &m : res].
-proof. by byequiv => //; proc; inline *; wp; swap{2} [1 .. 4] 3; sim. qed.
+proof. 
+byequiv => //; proc; inline *. 
+by wp;sim;auto => />.
+qed.
 
 local lemma rom_reprogramming1 &m i_ : 
      0 <= i_ 
@@ -926,20 +926,20 @@ local lemma rom_reprogramming1 &m i_ :
      <= 
      query_ctr%r * p_max_bound.
 proof.
-move=> hi; rewrite (Hip1_Hi1 &m i_) (Hi1_ERO_LRO  &m i_) (Hi1_LRO_Hi2 &m i_).
-rewrite -(Hi4_Hi &m i_) -(Hi4_LRO_ERO &m i_) -(Hi3_Hi4 &m i_) 1://.
+move=> hi; rewrite (Hip1_Hi1 &m i_) (Hi1_FunRO_RO  &m i_) (Hi1_LRO_Hi2 &m i_).
+rewrite -(Hi4_Hi &m i_) -(Hi4_RO_FunRO &m i_) -(Hi3_Hi4 &m i_) 1://.
 by move: (Hi2_Hi3 &m i_) (Hi2_bad &m i_) (Hi3_bad &m i_) => /#.
 qed.
 
 (* ----------------------------------------------------- *)
 
 lemma Bound_IND_Repro &m : 
-     hoare[A(O_Programmable(ERO), O_Reprogrammer(O_Programmable(ERO))).distinguish : 
+     hoare[A(O_Programmable(FunRO), O_Reprogrammer(O_Programmable(FunRO))).distinguish : 
              O_Programmable.ch = 0 /\ O_Reprogrammer.ctr = 0 /\ O_Reprogrammer.se 
              ==> O_Programmable.ch <= query_ctr /\ 
              O_Reprogrammer.ctr <= rep_ctr /\ O_Reprogrammer.se]
-  => `| Pr[IND_Repro(ERO, A).main(false) @ &m : res] - 
-        Pr[IND_Repro(ERO, A).main(true) @ &m : res] |
+  => `| Pr[IND_Repro(FunRO, A).main(false) @ &m : res] - 
+        Pr[IND_Repro(FunRO, A).main(true) @ &m : res] |
       <= 
       rep_ctr%r * query_ctr%r * p_max_bound. 
 proof.
@@ -969,16 +969,15 @@ end Adaptive.
 theory NonAdaptive.
 
 module type Oracleip_t = {
-  include Oracle
+  include RO [ init, get, set]
   proc oc(x : in_t) : out_t
-  proc set(x : in_t, y : out_t) : unit
 }.
 
 module type Oraclep_t = {
   include Oracleip_t [-init]
 }.
 
-module O_Programmable(O : POracle) : Oraclep_t = {
+module O_Programmable(O : RO) : Oraclep_t = {
    var prog_list : (in_t * out_t) list  
    var ch : int
 
@@ -987,11 +986,11 @@ module O_Programmable(O : POracle) : Oraclep_t = {
      ch <- 0;
    }
 
-  proc o(x : in_t): out_t = {
+  proc get(x : in_t): out_t = {
     var r,c : out_t;
     var tmp : out_t option;
 
-    r <@ O.o(x);
+    r <@ O.get(x);
 
     tmp <- assoc prog_list x;
     c <- if tmp = None then r else oget tmp;
@@ -1004,7 +1003,7 @@ module O_Programmable(O : POracle) : Oraclep_t = {
     
     ch <- ch + 1;
     
-    c <@ o(x);
+    c <@ get(x);
     
     return c;
   }
@@ -1016,10 +1015,10 @@ module O_Programmable(O : POracle) : Oraclep_t = {
 
 module type Adv_INDNARepro(O : Oraclep_t) = {
   proc pick() : pT list {O.oc}
-  proc distinguish(xs : in_t list) : bool {O.o}
+  proc distinguish(xs : in_t list) : bool {O.get}
 }.
 
-module IND_NARepro(O : Oracle, A : Adv_INDNARepro) = {
+module IND_NARepro(O : RO, A : Adv_INDNARepro) = {
   module OP = O_Programmable(O)
  
   proc main(b : bool, n : int) : bool = {
@@ -1062,18 +1061,18 @@ Then, IND_NARepro(true) with RO = IND_NARepro(true) with LRO = IND_NARepro(false
 *)
 section.
 
-declare module A <: Adv_INDNARepro {-IND_NARepro, -ERO}.
+declare module A <: Adv_INDNARepro {-IND_NARepro, -FunRO}.
 
 declare op rep_ctr : { int | 0 <= rep_ctr } as ge0_repctr.
 declare op query_ctr : { int | 0 <= query_ctr } as ge0_queryctr.
 
 lemma Bound_IND_NARepro &m : 
-     hoare[A(O_Programmable(ERO)).pick : 
+     hoare[A(O_Programmable(FunRO)).pick : 
              O_Programmable.ch = 0 
              ==> 
              O_Programmable.ch <= query_ctr /\ all ((>=) p_max_bound) (map p_max res)]
-  => `| Pr[IND_NARepro(ERO, A).main(false, rep_ctr) @ &m : res] - 
-        Pr[IND_NARepro(ERO, A).main(true, rep_ctr) @ &m : res] |
+  => `| Pr[IND_NARepro(FunRO, A).main(false, rep_ctr) @ &m : res] - 
+        Pr[IND_NARepro(FunRO, A).main(true, rep_ctr) @ &m : res] |
       <= 
       rep_ctr%r * query_ctr%r * p_max_bound.
 proof.
